Stuff in FutureCardinality.thy

Launchbury/CallFutureCardinality.thy
@@ -1,15 +1,82 @@
 theory CallFutureCardinality
-imports Vars "Cardinality-Domain"
+imports Vars "Cardinality-Domain" "Set-Cpo"
 begin
 
+fun no_call_in_path where
+  "no_call_in_path x [] \<longleftrightarrow> True"
+ | "no_call_in_path x (y#xs) \<longleftrightarrow> y \<noteq> x \<and> no_call_in_path x xs"
+
+fun one_call_in_path where
+  "one_call_in_path x [] \<longleftrightarrow> True"
+ | "one_call_in_path x (y#xs) \<longleftrightarrow> (if x = y then no_call_in_path x xs else one_call_in_path x xs)"
+
+
+lemma no_call_in_tail: "no_call_in_path x (tl p) \<longleftrightarrow> (no_call_in_path x p \<or> one_call_in_path x p \<and> hd p = x)"
+  by(induction p) auto
+
+lemma no_imp_one: "no_call_in_path x p \<Longrightarrow> one_call_in_path x p"
+  by (induction p) auto
+
+lemma one_imp_one_tail: "one_call_in_path x p \<Longrightarrow> one_call_in_path x (tl p)"
+  by (induction p) (auto split: if_splits intro: no_imp_one)
+
+(*
+lemma many_tail_imp_many: "\<not> one_call_in_path x (tl p) \<Longrightarrow> \<not> one_call_in_path x p"
+  by (induction p) auto
+*)
+
+
 definition pathCard :: "var list  \<Rightarrow> (var \<Rightarrow> two)"
-  where "pathCard f x = (if x \<notin> set f then none else (if length (filter (\<lambda> y. x = y) f) = 1 then once else many))"
+  where "pathCard p x = (if no_call_in_path x p then none else (if one_call_in_path x p then once else many))"
+
+lemma pathCard_Nil[simp]: "pathCard [] = \<bottom>"
+   by rule (simp add: pathCard_def)
+
+lemma pathCard_Cons[simp]: "pathCard (x#xs) x = two_add\<cdot>once\<cdot>(pathCard xs x)"
+  unfolding pathCard_def
+  by (auto simp add: two_add_simp)
+
+lemma pathCard_Cons_other[simp]: "x' \<noteq> x \<Longrightarrow> pathCard (x#xs) x' = pathCard xs x'"
+  unfolding pathCard_def by auto
+
 
 definition pathsCard :: "var list set \<Rightarrow> (var \<Rightarrow> two)"
-  where "pathsCard fs x = lub ((\<lambda> f. pathCard f x)` fs )"
+  where "pathsCard ps x = (if (\<forall> p \<in> ps. no_call_in_path x p) then none else (if (\<forall> p\<in>ps. one_call_in_path x p) then once else many))"
 
 lemma paths_Card_above:
-  "f \<in> fs \<Longrightarrow> pathCard f \<sqsubseteq> pathsCard fs"
-  sorry
+  "p \<in> ps \<Longrightarrow> pathCard p \<sqsubseteq> pathsCard ps"
+  by (rule fun_belowI) (auto simp add: pathsCard_def pathCard_def)
+
+lemma pathsCard_below:
+  assumes  "\<And> p. p \<in> ps \<Longrightarrow> pathCard p \<sqsubseteq> ce"
+  shows "pathsCard ps \<sqsubseteq> ce"
+proof(rule fun_belowI)
+  fix x
+  show "pathsCard ps x \<sqsubseteq> ce x"
+    by (auto simp add: pathsCard_def pathCard_def split: if_splits dest!: fun_belowD[OF assms, where x = x] elim: below_trans[rotated] dest: no_imp_one)
+qed
+
+lemma pathsCard_mono:
+  "ps \<subseteq> ps' \<Longrightarrow> pathsCard ps \<sqsubseteq> pathsCard ps'"
+  by (auto intro: pathsCard_below paths_Card_above)
+
+lemmas pathsCard_mono' = pathsCard_mono[folded below_set_def]
+
+lemma record_call_pathsCard: 
+  "pathsCard ({ tl p | p . p \<in> fs \<and> hd p = x}) \<sqsubseteq> record_call x\<cdot>(pathsCard fs)"
+proof (rule pathsCard_below)
+  fix p'
+  assume "p' \<in> {tl p |p. p \<in> fs \<and> hd p = x}"
+  then obtain p where "p' = tl p" and "p \<in> fs" and "hd p = x" by auto
+  
+  have "pathCard (tl p) \<sqsubseteq> record_call x\<cdot>(pathCard p)"
+    apply (rule fun_belowI)
+    using `hd p = x` by (auto simp add: pathCard_def record_call_simp no_call_in_tail dest: one_imp_one_tail)
+    
+  hence "pathCard (tl p) \<sqsubseteq> record_call x\<cdot>(pathsCard fs)"
+    by (rule below_trans[OF _ monofun_cfun_arg[OF  paths_Card_above[OF `p \<in> fs`]]])
+  thus "pathCard p' \<sqsubseteq> record_call x\<cdot>(pathsCard fs)" using `p' = _` by simp
+qed
+  
 
 end
